Clean up key-expansion-interleaving proofs (#333)

silveroak-opentitan/aes/Spec/InterleavedCipher.v
@@ -25,16 +25,15 @@ Require Import AesSpec.Cipher.
 Require Import AesSpec.ExpandAllKeys.
 
 Section Spec.
-  Context {state key rconst : Type}
+  Context {state key : Type}
           (add_round_key : state -> key -> state)
           (sub_bytes shift_rows mix_columns : state -> state)
-          (inv_sub_bytes inv_shift_rows inv_mix_columns : state -> state)
-          (inv_mix_columns_key : key -> key)
-          (key_expand : nat -> rconst -> key -> rconst * key).
+          (key_expand : nat -> key -> key).
 
   Definition cipher_round_interleaved
-             (rcon : rconst) (round_key : key) (st : state) (i : nat)
-    : rconst * key * state :=
+             (loop_state : key * state) (i : nat)
+    : key * state :=
+    let '(round_key, st) := loop_state in
     let st := if i =? 0
               then add_round_key st round_key
               else
@@ -43,47 +42,36 @@ Section Spec.
                 let st := mix_columns st in
                 let st := add_round_key st round_key in
                 st in
-    let rcon_key := key_expand i rcon round_key in
-    (rcon_key, st).
+    let round_key := key_expand i round_key in
+    (round_key, st).
 
-  (* AES cipher with interleaved key expansion and conditional split on first round *)
+  (* AES cipher with interleaved key expansion and conditional for first round *)
   Definition cipher_interleaved
              (Nr : nat) (* number of rounds *)
              (initial_key : key)
-             (initial_rcon : rconst)
              (input : state) : state :=
     let st := input in
     let loop_end_state :=
-        fold_left
-          (fun (loop_state : rconst * key * state) =>
-             let '(rcon, round_key, st) := loop_state in
-             cipher_round_interleaved rcon round_key st)
-          (List.seq 0 Nr)
-          (initial_rcon, initial_key, st) in
-    let '(_, last_key, st) := loop_end_state in
+        fold_left cipher_round_interleaved
+          (List.seq 0 Nr) (initial_key, st) in
+    let '(last_key, st) := loop_end_state in
     let st := sub_bytes st in
     let st := shift_rows st in
     let st := add_round_key st last_key in
     st.
 
   Section Equivalence.
-    Context (key_alt : Type) (* allow cipher to have a different type for keys *)
-            (projkey : key -> key_alt) (* convert to alternative key rep *)
-            (Nr : nat) (initial_rcon : rconst) (initial_key : key)
-            (first_key : key_alt) (middle_keys : list key_alt) (last_key : key_alt)
-            (add_round_key_alt : state -> key_alt -> state)
-            (add_round_key_alt_equiv :
-               forall st k, add_round_key_alt st (projkey k) = add_round_key st k)
-            (all_keys_eq :
-               List.map projkey
-                        (all_keys key_expand Nr initial_key initial_rcon)
+    Context (Nr : nat) (initial_key : key)
+            (first_key : key) (middle_keys : list key) (last_key : key).
+    Context (all_keys_eq :
+               all_keys key_expand Nr initial_key
                = first_key :: middle_keys ++ [last_key]).
 
-    Let cipher := cipher state key_alt add_round_key_alt sub_bytes shift_rows mix_columns.
+    Let cipher := cipher state key add_round_key sub_bytes shift_rows mix_columns.
 
     (* Interleaved cipher is equivalent to original cipher *)
     Lemma cipher_interleaved_equiv input :
-      cipher_interleaved Nr initial_key initial_rcon input =
+      cipher_interleaved Nr initial_key input =
       cipher first_key last_key middle_keys input.
     Proof.
       intros. subst cipher.
@@ -95,15 +83,13 @@ Section Spec.
                       rename H into Hall_keys end.
 
       cbv [cipher_interleaved cipher_round_interleaved Cipher.cipher].
-      (* pick the initial key as the default for nth_default *)
-      let x := lazymatch type of Hall_keys with all_keys _ _ ?k _ = _ => k end in
-      rewrite fold_left_to_seq with (default:=projkey x).
-      pose proof (length_all_keys _ _ _ _ _ _ Hall_keys).
+      rewrite fold_left_to_seq with (default:=initial_key).
+      pose proof (length_all_keys _ _ _ _ _ Hall_keys).
       autorewrite with push_length in *.
 
       (* Nr cannot be 0 *)
       destruct Nr as [|Nr_m1]; [ lia | ].
-      pose proof (hd_all_keys _ _ _ _ _ _ Hall_keys ltac:(lia)).
+      pose proof (hd_all_keys _ _ _ _ _ Hall_keys ltac:(lia)).
       subst.
       match goal with
       | H : length ?x + 1 = S ?n |- context [length ?x] =>
@@ -116,10 +102,10 @@ Section Spec.
 
       (* state the relationship between the two loop states (invariant) *)
       lazymatch goal with
-      | H : all_keys ?key_expand ?n ?k ?r = _ |- _ =>
-        pose (R:= fun (i : nat) (x : rconst * key * state) (y : state) =>
+      | H : all_keys ?key_expand ?n ?k = _ |- _ =>
+        pose (R:= fun (i : nat) (x : key * state) (y : state) =>
                     x = (nth (S i)
-                             (all_rcons_and_keys key_expand n k r) (r,k), y))
+                             (all_keys key_expand n k) k, y))
       end.
 
       (* find loops on each side *)
@@ -140,9 +126,7 @@ Section Spec.
         (* prove that if the invariant is satisfied at the end of the loop, the
            postcondition is true *)
         repeat destruct_pair_let.
-        rewrite <-add_round_key_alt_equiv.
         f_equal; [ ].
-        rewrite nth_all_rcons_and_keys_all_keys.
         rewrite Hall_keys, app_comm_cons.
         rewrite app_nth2 by length_hammer.
         match goal with |- context [nth ?i _ _] =>
@@ -152,23 +136,17 @@ Section Spec.
       (* use the fold_left invariant lemma *)
       apply fold_left_preserves_relation_seq with (R0:=R); subst R.
       { (* invariant holds at loop start *)
-        cbv beta. rewrite nth_all_rcons_and_keys by lia.
-        rewrite add_round_key_alt_equiv.
+        cbv beta. rewrite nth_all_keys by lia.
         reflexivity. }
       { (* invariant holds through loop step *)
         cbv beta; intros; subst. repeat destruct_pair_let.
         rewrite Nat.eqb_compare; cbn [Nat.compare].
-        rewrite !nth_all_rcons_and_keys_succ by lia.
-        rewrite <-add_round_key_alt_equiv.
-        f_equal; [ ]. rewrite map_nth.
-        lazymatch goal with
-        | H : @eq (list key) ?ls (_ :: (?m ++ [_]))%list
-          |- context [@nth key ?i ?mk ?d] =>
-          replace (nth i mk d) with (nth (S i) ls d)
-            by (rewrite H; apply app_nth1; Lia.lia)
-        end.
-        rewrite <-nth_all_rcons_and_keys_all_keys.
-        rewrite !nth_all_rcons_and_keys_succ by lia.
+        f_equal;
+          [ rewrite !nth_all_keys_succ by lia;
+            reflexivity | ].
+        f_equal; [ ].
+        rewrite Hall_keys. cbn [nth].
+        rewrite app_nth1 by length_hammer.
         reflexivity. }
     Qed.
   End Equivalence.
