silveroak-opentitan/aes/Arrow/OpenTitanCipherEquivalence.v
@@ -27,6 +27,7 @@ Require Import Cava.ListUtils.
 Require Import Cava.Tactics.
 Require Import Cava.VectorUtils.
 Require Import AesSpec.Cipher.
+Require Import AesSpec.CipherRepresentationChange.
 Require Import AesSpec.ExpandAllKeys.
 Require Import AesSpec.InterleavedCipher.
 From Aes Require Import OpenTitanCipherProperties CipherRoundProperties
@@ -72,8 +73,8 @@ Section Equivalence.
   Definition shift_rows : state -> state := aes_shift_rows_spec false.
   Definition mix_columns : state -> state := aes_mix_columns_spec false.
 
-  Definition key_expand : nat -> rconst -> keypair -> rconst * keypair :=
-    fun i => aes_key_expand_spec sbox false (nat_to_bitvec _ i).
+  Definition key_expand : nat -> rconst * keypair -> rconst * keypair :=
+    fun i rk => aes_key_expand_spec sbox false (nat_to_bitvec _ i) (fst rk) (snd rk).
 
   Definition fstkey : keypair -> key :=
     @slice_by_position
@@ -88,18 +89,31 @@ Section Equivalence.
     let init_rcon := nat_to_byte 1 in
     (* initial key pair reversed so key_expand doesn't have to mux *)
     let init_keypair_rev := sndkey init_keypair ++ fstkey init_keypair in
-    let all_keypairs := all_keys key_expand Nr init_keypair_rev init_rcon in
-    (* project out the forward key from the pair and transpose it *)
-    let all_keys := List.map (fun kp => PkgProperties.Vector.transpose_rev (sndkey kp))
-                             all_keypairs in
+    (* key_expand state is rconst * keypair *)
+    let init_rk := (init_rcon, init_keypair_rev) in
+    let all_rcons_and_keypairs := all_keys key_expand Nr init_rk in
+    (* representation change: project out the forward key and transpose it *)
+    let all_keys := List.map (fun x : rconst * keypair =>
+                                PkgProperties.Vector.transpose_rev (sndkey (snd x)))
+                             all_rcons_and_keypairs in
     all_keys = (first_key :: middle_keys ++ [last_key])%list ->
     unrolled_cipher_spec aes_key_expand_spec sbox false input init_keypair
     = cipher state key add_round_key sub_bytes shift_rows mix_columns
              first_key last_key middle_keys input.
   Proof.
-    cbv zeta. cbn [denote_kind] in *. intros.
-    erewrite <-cipher_interleaved_equiv
-      by (eassumption || intros; instantiate_app_by_reflexivity).
+    cbv zeta. cbn [denote_kind] in *. intro Hall_keys.
+
+    (* Get all states from key expansion *)
+    map_inversion Hall_keys; subst.
+    match goal with H : @eq (list (_ * keypair)) _ (_ :: _ ++ [_])%list |- _ =>
+                    rename H into Hall_keys end.
+
+    (* representation change; use full key-expansion state (rconst * keypair) *)
+    erewrite cipher_change_key_rep with
+        (projkey := fun x => PkgProperties.Vector.transpose_rev (sndkey (snd x)))
+      by reflexivity.
+
+    erewrite <-cipher_interleaved_equiv by eassumption.
     cbv [unrolled_cipher_spec final_cipher_round_spec
                               cipher_interleaved cipher_round_interleaved].
     repeat destruct_pair_let.
