silveroak-opentitan/aes/Spec/CipherRepresentationChange.v
@@ -1,0 +1,44 @@
+(* Copyright 2020 The Project Oak Authors                                   *)
+(*                                                                          *)
+(* Licensed under the Apache License, Version 2.0 (the "License")           *)
+(* you may not use this file except in compliance with the License.         *)
+(* You may obtain a copy of the License at                                  *)
+(*                                                                          *)
+(*     http://www.apache.org/licenses/LICENSE-2.0                           *)
+(*                                                                          *)
+(* Unless required by applicable law or agreed to in writing, software      *)
+(* distributed under the License is distributed on an "AS IS" BASIS,        *)
+(* WITHOUT WARRANTIES OR CONDITIONS OF ANY KIND, either express or implied. *)
+(* See the License for the specific language governing permissions and      *)
+(* limitations under the License.                                           *)
+(****************************************************************************)
+
+Require Import Coq.Lists.List.
+Require Import Cava.ListUtils.
+Require Import AesSpec.Cipher.
+
+Section ChangeKeyRepresentation.
+  Context (state key key_alt : Type)
+          (projkey : key_alt -> key)
+          (add_round_key : state -> key -> state)
+          (sub_bytes shift_rows mix_columns : state -> state)
+          (inv_sub_bytes inv_shift_rows inv_mix_columns : state -> state)
+          (inv_mix_columns_key : key -> key).
+
+  Lemma cipher_change_key_rep first_key last_key middle_keys
+        first_key_alt last_key_alt middle_keys_alt input :
+    projkey first_key_alt = first_key ->
+    projkey last_key_alt = last_key ->
+    map projkey middle_keys_alt = middle_keys ->
+    cipher state key add_round_key sub_bytes shift_rows mix_columns
+           first_key last_key middle_keys input
+    = cipher state key_alt (fun st k => add_round_key st (projkey k))
+             sub_bytes shift_rows mix_columns first_key_alt last_key_alt
+             middle_keys_alt input.
+  Proof.
+    intros; subst; cbv [cipher].
+    repeat (f_equal; [ ]).
+    rewrite fold_left_map.
+    reflexivity.
+  Qed.
+End ChangeKeyRepresentation.
